First pass of expression evaluation in semantics.

Semantics.v
@@ -5,7 +5,61 @@ Require Import Coq.FSets.FMapInterface.
 
 Module Semantics (Map : WSfun).
 
+Module Program := Program Map.
+
 Module Heap := Heap Map.
 Include Heap.
+
+Inductive evaluatesTo { P : Program.program } : forall (X : Type), heap -> localVars -> X -> heap -> localVars -> value -> Prop :=
+  | eval_local (chi : heap) (L : localVars) (x : Syntax.var) (v : value)
+  : VarMap.MapsTo x v L
+    -> evaluatesTo Syntax.path chi L (Syntax.use x) chi L v
+  | eval_consume (chi : heap) (L : localVars) (x : Syntax.var) (v : value)
+  : VarMap.MapsTo x v L
+    -> evaluatesTo Syntax.path chi L (Syntax.consume x) chi (VarMap.remove x L) v
+  | eval_field (chi chi' : heap) (L L' : localVars) (p : Syntax.path) (f : Syntax.fieldId) (v v' : value)
+  : evaluatesTo Syntax.path chi L p chi' L' v
+    -> HeapFieldLookup v f v' chi'
+    -> evaluatesTo Syntax.fieldOfPath chi L (p, f) chi' L' v'
+  | eval_alias (chi chi' : heap) (L L' : localVars) (X : Type) (x : X) (v : value)
+  : evaluatesTo X chi L x chi' L' v
+    -> evaluatesTo (@Syntax.aliased X) chi L (Syntax.aliasOf x) chi' L' v
+  | eval_vardecl (chi : heap) (L : localVars) (x : Syntax.var)
+  : evaluatesTo Syntax.expression chi L (Syntax.varDecl x) chi (VarMap.add x None L) None
+  | eval_localassign (chi chi' : heap) (L L' : localVars) (x : Syntax.var) (arhs : @Syntax.aliased Syntax.rhs) (v v' : value)
+  : evaluatesTo Syntax.aliased chi L arhs chi' L' v
+    -> VarMap.MapsTo x v' L'
+    -> evaluatesTo Syntax.expression chi L (Syntax.assign x arhs) chi' (VarMap.add x v L') v'
+  | eval_fieldassign (chi chi' chi'' chi''' : heap) (L L' L'' : localVars) (p : Syntax.path) (f : Syntax.fieldId)
+    (ap : @Syntax.aliased Syntax.path) (u v v' : value)
+  : evaluatesTo Syntax.aliased chi L ap chi' L' v
+    -> evaluatesTo Syntax.path chi' L' p chi'' L'' u
+    -> HeapFieldLookup u f v' chi''
+    -> HeapFieldAdd u f v chi'' chi'''
+    -> evaluatesTo Syntax.rhs chi L (Syntax.fieldAssign (p, f) ap) chi''' L'' v'
+  | eval_becall (chi chi' chi'' : heap) (L L' L'' : localVars) (rcvr : @Syntax.aliased Syntax.path) (args : list (@Syntax.aliased Syntax.path))
+    (b : Syntax.behaviourId) (rcvrVal : value) (argVals : list value)
+  : evaluatesTo_list Syntax.aliased chi L args chi' L' argVals
+    -> evaluatesTo Syntax.aliased chi' L' rcvr chi'' L'' rcvrVal
+    -> False (*TODO: receiver is actor in the heap *)
+    -> False (*TODO: append message to queue *)
+    -> evaluatesTo Syntax.rhs chi L (Syntax.behaviourCall rcvr b args) chi'' L'' rcvrVal
+with
+evaluatesTo_list { P : Program.program } : forall (X : Type), heap -> localVars -> list X -> heap -> localVars -> list value -> Prop :=
+  | evaluatesTo_list_nil (X : Type) (chi : heap) (L : localVars)
+  : evaluatesTo_list X chi L nil chi L nil
+  | evaluatesTo_list_cons (X: Type) (chi chi' chi'' : heap) (L L' L'' : localVars) (x : X) (lx : list X) (v : value) (lv : list value)
+  : evaluatesTo X chi L x chi' L' v
+    -> evaluatesTo_list X chi' L' lx chi'' L'' lv
+    -> evaluatesTo_list X chi L (x :: lx) chi'' L'' (v :: lv).
+
+Lemma paths_dont_change_heap { P : Program.program } : forall chi chi' L L' p v, @evaluatesTo P Syntax.path chi L p chi' L' v -> chi = chi'.
+Proof.
+  intros.
+  inversion H; try reflexivity.
+  (* TODO: get axioms for these inequalities *)
+  admit.
+  admit.
+  Admitted.
 
 End Semantics.
